Start module

src/Knapsack/Module.dfy
@@ -1,6 +1,6 @@
 //include "Implementation/Solution.dfy"
 
-abstract module Q {
+module Q {
     class Solution {
         var priority : real
 
@@ -16,17 +16,137 @@ abstract module Q {
     */
     class PriorityQueue {
         var arr : array<Solution>
-        var size : int // fixed size of arr
+        var count : int  // current number of elements, if count == arr.Length, array must grow
 
-        constructor PriorityQueue(arr': array<Solution>, size': int)
-            ensures this.arr == arr'
-            ensures this.size == size'
+
+        constructor PriorityQueue(size: int)
+            //ensures this.IsHeap()
         {
-            this.arr := arr';
-            this.size := size';
+            this.arr := new Solution[0];
+            this.count := 0;
         }
 
-        //methods
+
+        /* Predicates */
+
+        /* Predicate: true if the array satisfies the heap property */
+        predicate IsHeap() 
+            reads this, this.arr, set i | 0 <= i < this.arr.Length :: arr[i]
+        {
+            && 0 <= this.count <= arr.Length
+            && (forall i | 0 < i < this.count :: this.arr[(i-1)/2].priority < this.arr[i].priority)
+        }
+
+        /* Predicate: true if the heap has no elements */
+        predicate IsEmpty()
+            reads this
+        {
+            this.count == 0
+        }
+
+
+
+        /* Methods */
+
+        /* Method: return the maximum capacity of the heap */
+        method Size() returns (s : int)
+        {
+            return this.arr.Length;
+        }
+
+
+        /* Method: returns the current number of elements in the heap */
+        method Count() returns (c : int)
+        {
+            return this.count;
+        }
+
+
+        /* Method: returns the element with the minimum priority in the heap */
+        method Min() returns (m : Solution)
+            requires 0 < this.count <= this.arr.Length <= this.arr.Length
+            requires this.IsHeap()
+        {
+            return this.arr[0];
+        }
+
+        
+        /* Method: inserts an element to the heap */
+        method Insert(node : Solution)
+            modifies this, this.arr
+            requires this.IsHeap()
+            requires 0 < this.arr.Length == this.arr.Length
+            ensures this.IsHeap()
+        {
+            if (this.count == this.arr.Length) {
+                Grow(node);
+            }
+            this.count := this.count + 1;
+            this.Float();     
+        }
+
+        /* Method: duplicates space of the heap */
+        method Grow(x : Solution)
+            modifies this, this.arr
+            requires 0 <= this.count == this.arr.Length
+            ensures this.count == old(this.count) // el numero de elementos no aumenta, lo hace Insert
+            ensures this.arr[0..this.count] == old(this.arr[0..this.count]) // los primeros elementos que habia antes en el array se conservan
+            ensures this.arr.Length > old(this.arr.Length) // la longitud aumenta
+            ensures fresh(this.arr) // es nuevo en la memoria
+        {
+            // allocate new memory
+            var aux: array<Solution> := new Solution[2 * this.arr.Length + 1] (_ => x);
+            
+            assert this.count == this.arr.Length;
+            // copy
+            var i := 0;
+            while i < this.count
+                decreases this.count-i
+                invariant 0 <= i <= this.count <= this.arr.Length < aux.Length && this.count == old(this.count)
+                invariant aux[0..i] == this.arr[0..i]
+                invariant this.arr[0..this.count] == old(this.arr[0..this.count])
+            {
+                aux[i] := this.arr[i];
+                i := i + 1;
+            }
+            assert aux[0..this.count] == this.arr[0..this.count] == old(this.arr[0..this.count]);
+            //assert Seq.Rev(aux[0..size]) == Seq.Rev(list[0..size]) == Seq.Rev(old(list[0..size]));
+            this.arr := aux;
+            //assert Model() == Seq.Rev(aux[0..size]);
+        }
+
+
+        /* Method: */
+        method Float()
+            modifies this.arr
+            requires 0 < this.count <= this.arr.Length
+            requires forall i | 0 < i < this.count - 1 :: this.arr[(i-1)/2].priority <= this.arr[i].priority
+            ensures this.IsHeap()
+        
+
+
+
+        /* Method: returns the element with the minimum priority of the heap */
+        method DeleteMin()
+            modifies this, this.arr
+            requires this.IsHeap()
+            requires 0 < this.count
+            //ensures this.IsHeap()
+        {
+            this.arr[0] := this.arr[this.count - 1];
+            this.count := this.count - 1;
+            //Sink(0, this.count);
+        }
+
+
+        /* Method: the element with the minimum priority of the heap */
+        method Sink(s : nat, l : nat)
+            modifies this.arr
+            requires 0 <= s <= l == this.count <= arr.Length
+            requires forall i | 0 < i < this.count && (i-1)/2 != s :: this.arr[(i-1)/2].priority <= this.arr[i].priority
+            ensures this.IsHeap()
+        
+
 
         
     }
